switching the exercises to use FStar.Integers overloading

courses/fstar-sri-2018/LabSession.fst
@@ -3,10 +3,9 @@ module LabSession
 /// Lab Session: Programming in Low*. This is intended as a warm-up to get
 /// familiar with Low*. The module defines a few aliases that may come in handy.
 module B = LowStar.Buffer
-module U32 = FStar.UInt32
-module I32 = FStar.Int32
 module HS = FStar.HyperStack
 
+open FStar.Integers
 open LowStar.BufferOps
 open FStar.HyperStack.ST
 open LowStar.Modifies
@@ -21,7 +20,7 @@ let abs (x: int): Tot int = if x > 0 then x else -x
 
 /// In order to move forward, you will need the definition of the smallest
 /// representable signed 32-bit integer.
-let min_int32 = I32.(0l -^ 0x7fffffffl -^ 1l)
+let min_int32 = -0x7fffffffl - 1l
 
 /// Then show that our function that operates on machine integers performs that
 /// operation properly. Remember that computations over machine integers are
@@ -29,15 +28,14 @@ let min_int32 = I32.(0l -^ 0x7fffffffl -^ 1l)
 /// - no unary minus
 /// - local open syntax I32.( ... )
 /// - arithmetic operations are suffixed with ^
-let abs1 (x: Int32.t): Pure Int32.t
+let abs1 (x: int_32): Pure int_32
   (requires True) // enhance this pre-condition
   (ensures (fun _ -> True)) // enhance this post-condition to use abs above
-=
-  admit ()
+= admit ()
 
 /// A second variant: this one will take True as a precondition, but will return
 /// an option type for those inputs whose absolute value cannot be computed.
-let abs2 (x: Int32.t): Pure (option Int32.t)
+let abs2 (x: int_32): Pure (option int_32)
   (requires True) // must leave True here
   (ensures (fun _ -> True))
 =
@@ -54,7 +52,7 @@ let abs2 (x: Int32.t): Pure (option Int32.t)
 /// - modifies l h0 h1, a predicate stating that going from memory h0 to memory
 ///   h1, only location l was modified.
 /// - B.get h p i, which fetches the contents of pointer p in heap h at index i
-let swap (x: B.pointer UInt32.t) (y: B.pointer UInt32.t): Stack unit
+let swap (x: B.pointer uint_32) (y: B.pointer uint_32): Stack unit
   (requires fun h0 -> B.live h0 x /\ B.live h0 y /\ B.disjoint x y)
   (ensures fun _ _ _ -> True)
 =
@@ -69,30 +67,27 @@ let swap (x: B.pointer UInt32.t) (y: B.pointer UInt32.t): Stack unit
 
 /// Our first useful definition is a type abbreviation for a buffer whose length
 /// is known at type-checking time.
-let lbuffer (len:U32.t) (a:Type) = b:B.buffer a{U32.(len <=^ B.len b)}
+let lbuffer (len:uint_32) (a:Type) = b:B.buffer a{len <= B.len b}
 
 /// A predicate, stating that b1 and b2 are equal, in memory h, over their first
 /// i elements.
-let prefix_equal (#l:U32.t) (#a:Type) (h:HS.mem) (b1 b2: lbuffer l a) (i:U32.t{U32.(i <=^ l)}) =
-  forall (j:nat). j < U32.v i ==> B.get h b1 j == B.get h b2 j
+let prefix_equal (#l:uint_32) (#a:Type) (h:HS.mem) (b1 b2: lbuffer l a) (i:uint_32{i <= l}) =
+  forall (j:nat). j < v i ==> B.get h b1 j == B.get h b2 j
 
 /// For this version, you are expected to verify safety, but also functional
 /// correctness. Start by writing the code, then proving that it is memory safe.
 /// Here is the list of predicates you will need:
 /// - B.live h b, to show that buffer b is live in memory h
 /// - B.disjoint b1 b2, to show that two buffers do not overlap
-/// - U32.( ... <=^ ... ), less-than-or-equal comparison for unsigned 32-bit ints
 /// - loc_buffer b, the injection of a buffer into the generic type of memory locations
 /// - modifies l h0 h1, a predicate stating that going from memory h0 to memory
 ///   h1, only location l was modified.
 /// Once you have proved memory safety, show how copy_correct extends the
 /// prefix_equal predicate.
-let rec copy_correct (#len:U32.t) (dst src:lbuffer len U32.t) (cur: U32.t): Stack unit
+let rec copy_correct (#len:uint_32) (dst src:lbuffer len uint_32) (cur: uint_32): Stack unit
   (requires fun h0 ->
-     let open U32 in
      True)
   (ensures fun h0 _ h1 ->
      True)
 =
-  let open U32 in
   admit ()
