courses/fstar-sri-2018/Solution.LabSession.fst
@@ -7,6 +7,7 @@ module U32 = FStar.UInt32
 module I32 = FStar.Int32
 module HS = FStar.HyperStack
 
+open FStar.Integers
 open LowStar.BufferOps
 open FStar.HyperStack.ST
 open LowStar.Modifies
@@ -21,7 +22,7 @@ let abs (x: int): Tot int = if x > 0 then x else -x
 
 /// In order to move forward, you will need the definition of the smallest
 /// representable signed 32-bit integer.
-let min_int32 = I32.(0l -^ 0x7fffffffl -^ 1l)
+let min_int32 = -0x7fffffffl - 1l
 
 /// Then show that our function that operates on machine integers performs that
 /// operation properly. Remember that computations over machine integers are
@@ -29,17 +30,17 @@ let min_int32 = I32.(0l -^ 0x7fffffffl -^ 1l)
 /// - no unary minus
 /// - local open syntax I32.( ... )
 /// - arithmetic operations are suffixed with ^
-let abs1 (x: Int32.t): Pure Int32.t
+let abs1 (x: int_32): Pure int_32
   (requires x <> min_int32) // enhance this pre-condition
-  (ensures (fun y -> I32.v y = abs (I32.v x))) // enhance this post-condition to use abs above
+  (ensures (fun y -> v y = abs (v x))) // enhance this post-condition to use abs above
 = let open I32 in
-  if x <^ 0l then 0l -^ x else x
+  if x < 0l then 0l - x else x
 
 /// A second variant: this one will take True as a precondition, but will return
 /// an option type for those inputs whose absolute value cannot be computed.
-let abs2 (x: Int32.t): Pure (option Int32.t)
+let abs2 (x: int_32): Pure (option int_32)
   (requires True) // must leave True here
-  (ensures (function None -> x = min_int32 | Some y -> I32.v y = abs (I32.v x)))
+  (ensures (function None -> x = min_int32 | Some y -> v y = abs (v x)))
 = if x = min_int32 then None
   else Some (abs1 x)
 
@@ -47,7 +48,7 @@ let abs2 (x: Int32.t): Pure (option Int32.t)
 /// The classic swap on references: provide suitable pre- and post-conditions.
 /// Two useful operations: b *= (e), for writing into a pointer, and !*(e), for
 /// dereferencing a pointer.
-let swap (x: B.pointer UInt32.t) (y: B.pointer UInt32.t): Stack unit
+let swap (x: B.pointer uint_32) (y: B.pointer uint_32): Stack unit
   (requires fun h0 -> B.live h0 x /\ B.live h0 y /\ B.disjoint x y)
   (ensures fun h0 _ h1 ->
            modifies (loc_union (loc_buffer x) (loc_buffer y)) h0 h1 /\
@@ -67,40 +68,37 @@ let swap (x: B.pointer UInt32.t) (y: B.pointer UInt32.t): Stack unit
 
 /// Our first useful definition is a type abbreviation for a buffer whose length
 /// is known at type-checking time.
-let lbuffer (len:U32.t) (a:Type) = b:B.buffer a{U32.(len <=^ B.len b)}
+let lbuffer (len:uint_32) (a:Type) = b:B.buffer a{len <= B.len b}
 
 /// A predicate, stating that b1 and b2 are equal, in memory h, over their first
 /// i elements.
-let prefix_equal (#l:U32.t) (#a:Type) (h:HS.mem) (b1 b2: lbuffer l a) (i:U32.t{U32.(i <=^ l)}) =
-  forall (j:nat). j < U32.v i ==> B.get h b1 j == B.get h b2 j
+let prefix_equal (#l:uint_32) (#a:Type) (h:HS.mem) (b1 b2: lbuffer l a) (i:uint_32{i <= l}) =
+  forall (j:nat). j < v i ==> B.get h b1 j == B.get h b2 j
 
 /// For this version, you are expected to verify safety, but also functional
 /// correctness. Start by writing the code, then proving that it is memory safe.
 /// Here is the list of predicates you will need:
 /// - B.live h b, to show that buffer b is live in memory h
 /// - B.disjoint b1 b2, to show that two buffers do not overlap
-/// - U32.( ... <=^ ... ), less-than-or-equal comparison for unsigned 32-bit ints
 /// - loc_buffer b, the injection of a buffer into the generic type of memory locations
 /// - modifies l h0 h1, a predicate stating that going from memory h0 to memory
 ///   h1, only location l was modified.
 /// Once you have proved memory safety, show how copy_correct extends the
 /// prefix_equal predicate.
-let rec copy_correct (#len:U32.t) (dst src:lbuffer len U32.t) (cur: U32.t): Stack unit
+let rec copy_correct (#len:uint_32) (dst src:lbuffer len uint_32) (cur: uint_32): Stack unit
   (requires (fun h0 ->
-            let open U32 in
                 B.live h0 src 
               /\ B.live h0 dst
               /\ B.disjoint src dst
-              /\ cur <=^ len
+              /\ cur <= len
               /\ prefix_equal h0 src dst cur))
   (ensures fun h0 _ h1 ->
            B.live h1 src
            /\ B.live h1 dst
            /\ modifies (loc_buffer dst) h0 h1
            /\ prefix_equal h1 src dst len)
-= let open U32 in
-  if cur <> len
+= if cur <> len
   then begin
     dst.(cur) <- src.(cur);
-    copy_correct dst src (cur +^ 1ul)
+    copy_correct dst src (cur + 1ul)
  end
